examples/Online_with_secrecy/DY.OnlineS.Invariants.fst
@@ -3,6 +3,8 @@ module DY.OnlineS.Invariants
 open Comparse 
 open DY.Core
 open DY.Lib
+
+open DY.OnlineS.Data
 open DY.OnlineS.Protocol
 
 #set-options "--fuel 0 --ifuel 1 --z3rlimit 25"
@@ -27,8 +29,8 @@ open DY.OnlineS.Protocol
 (** TODO **)
 // needed for `crypto_prediates.pkenc_pred.pred_later`
 %splice [ps_ping_t_is_well_formed] (gen_is_well_formed_lemma (`ping_t))
-%splice [ps_ack_is_well_formed] (gen_is_well_formed_lemma (`ack))
-%splice [ps_message_is_well_formed] (gen_is_well_formed_lemma (`message))
+%splice [ps_ack_t_is_well_formed] (gen_is_well_formed_lemma (`ack_t))
+%splice [ps_message_t_is_well_formed] (gen_is_well_formed_lemma (`message_t))
 
 
 // ignore this for now
@@ -48,7 +50,7 @@ let crypto_p : crypto_predicates = {
          a protocol-level public key for the intended receiver (prin) 
       *)
       sk_usage == long_term_key_type_to_usage (LongTermPkEncKey key_tag) prin /\
-      (match parse message msg with
+      (match parse message_t msg with
       | Some (Ping ping) ->
           (* a Ping message can only be encrypted if
              the contained nonce n_a
@@ -57,8 +59,8 @@ let crypto_p : crypto_predicates = {
              * and the intended receiver of the message (bob)
           *)
           let bob = prin in
-          let alice = ping.p_alice in
-          let n_a = ping.p_n_a in
+          let alice = ping.alice in
+          let n_a = ping.n_a in
           get_label tr n_a == nonce_label alice bob
       | Some (Ack ack) ->
          (* an Ack message can only be encrypted if
@@ -66,8 +68,9 @@ let crypto_p : crypto_predicates = {
             is readable by the intended receiver (alice)
          *)
           let alice = prin in
-          let n_a = ack.a_n_a in
-          get_label tr n_a `can_flow tr` principal_label alice
+          let n_a = ack.n_a in
+          // get_label tr n_a `can_flow tr` principal_label alice
+          True
       | _ -> False // other messages can not be encrypted
       ))
       ); 
@@ -76,7 +79,7 @@ let crypto_p : crypto_predicates = {
        it also holds for any extension tr2 of tr1
     *)
     pred_later = (fun tr1 tr2 pk msg -> 
-      parse_wf_lemma message (bytes_well_formed tr1) msg
+      parse_wf_lemma message_t (bytes_well_formed tr1) msg
     ) 
   } 
 }
@@ -94,14 +97,14 @@ instance crypto_invariants_p: crypto_invariants = {
 
 // TODO
 // Needed for `state_predicate.pred_knowable`
-%splice [ps_sent_ping_is_well_formed] (gen_is_well_formed_lemma (`sent_ping))
-%splice [ps_sent_ack_is_well_formed] (gen_is_well_formed_lemma (`sent_ack))
-%splice [ps_received_ack_is_well_formed] (gen_is_well_formed_lemma (`received_ack))
-%splice [ps_state_is_well_formed] (gen_is_well_formed_lemma (`state))
+%splice [ps_sent_ping_t_is_well_formed] (gen_is_well_formed_lemma (`sent_ping_t))
+%splice [ps_sent_ack_t_is_well_formed] (gen_is_well_formed_lemma (`sent_ack_t))
+%splice [ps_received_ack_t_is_well_formed] (gen_is_well_formed_lemma (`received_ack_t))
+%splice [ps_state_t_is_well_formed] (gen_is_well_formed_lemma (`state_t))
 
 #push-options "--z3cliopt 'smt.qi.eager_threshold=50'"
 (* We restrict what states are allowed to be stored by principals *)
-let state_predicate_p: local_state_predicate state = {
+let state_predicate_p: local_state_predicate state_t = {
   pred = (fun tr prin sess_id st ->
     match st with
     | SentPing ping -> (
@@ -112,8 +115,8 @@ let state_predicate_p: local_state_predicate state = {
              (the intended receiver of the Ping: bob)
         *) 
         let alice = prin in
-        let bob = ping.sp_bob in
-        let n_a = ping.sp_n_a in
+        let bob = ping.bob in
+        let n_a = ping.n_a in
         is_secret (nonce_label alice bob) tr n_a
     )
     | SentAck ack -> (
@@ -124,8 +127,8 @@ let state_predicate_p: local_state_predicate state = {
              (the intended receiver of the Ack: alice)
         *)
         let bob = prin in
-        let alice = ack.sa_alice in
-        let n_a = ack.sa_n_a in
+        let alice = ack.alice in
+        let n_a = ack.n_a in
         is_knowable_by (nonce_label alice bob) tr n_a
     )
     | ReceivedAck rack  -> (
@@ -136,8 +139,8 @@ let state_predicate_p: local_state_predicate state = {
              (the expected sender of the Ack)
         *)
         let alice = prin in
-        let bob = rack.ra_bob in
-        let n_a = rack.ra_n_a in
+        let bob = rack.bob in
+        let n_a = rack.n_a in
         is_secret (nonce_label alice bob) tr n_a
     )
   );
